<?xml version="1.0"?>
<rdf:RDF xmlns="http://purl.org/ontology/UniOn#"
     xml:base="http://purl.org/ontology/UniOn"
     xmlns:uo="http://purl.org/ontology/UniOn#"
     xmlns:owl="http://www.w3.org/2002/07/owl#"
     xmlns:rdf="http://www.w3.org/1999/02/22-rdf-syntax-ns#"
     xmlns:xml="http://www.w3.org/XML/1998/namespace"
     xmlns:xsd="http://www.w3.org/2001/XMLSchema#"
     xmlns:rdfs="http://www.w3.org/2000/01/rdf-schema#">
    <owl:Ontology rdf:about="http://purl.org/ontology/UniOn">
        <owl:versionIRI rdf:resource="http://purl.org/ontology/UniOn/09-2022"/>
        <rdfs:comment>UniOn is an ontology representing Universities educational offer. It includes information to describe academic fields, degree programs, access methods and requirements, educational activities, titles and qualifications, location, organization and more</rdfs:comment>
    </owl:Ontology>
    


    <!-- 
    ///////////////////////////////////////////////////////////////////////////////////////
    //
    // Object Properties
    //
    ///////////////////////////////////////////////////////////////////////////////////////
     -->

    


    <!-- http://purl.org/ontology/UniOn#delivers -->

    <owl:ObjectProperty rdf:about="http://purl.org/ontology/UniOn#delivers">
        <owl:inverseOf rdf:resource="http://purl.org/ontology/UniOn#isDeliveredBy"/>
        <rdfs:domain rdf:resource="http://purl.org/ontology/UniOn#ItalianPublicUniversity"/>
        <rdfs:range rdf:resource="http://purl.org/ontology/UniOn#DegreeProgramme"/>
        <rdfs:comment>A property that relates an italian public university to the degree programmes it delivers.</rdfs:comment>
    </owl:ObjectProperty>
    


    <!-- http://purl.org/ontology/UniOn#hasAcademicField -->

    <owl:ObjectProperty rdf:about="http://purl.org/ontology/UniOn#hasAcademicField">
        <owl:inverseOf rdf:resource="http://purl.org/ontology/UniOn#isAcademicFieldOf"/>
        <rdfs:domain rdf:resource="http://purl.org/ontology/UniOn#DegreeProgramme"/>
        <rdfs:range rdf:resource="http://purl.org/ontology/UniOn#AcademicField"/>
        <rdfs:comment>A property linking the degree programme to the academic field to which it belongs.</rdfs:comment>
    </owl:ObjectProperty>
    


    <!-- http://purl.org/ontology/UniOn#hasAccessType -->

    <owl:ObjectProperty rdf:about="http://purl.org/ontology/UniOn#hasAccessType">
        <owl:inverseOf rdf:resource="http://purl.org/ontology/UniOn#isAccessTypeOf"/>
        <rdfs:domain rdf:resource="http://purl.org/ontology/UniOn#DegreeProgramme"/>
        <rdfs:range rdf:resource="http://purl.org/ontology/UniOn#AccessType"/>
        <rdfs:comment>A property relating the degree programme to the modality of access it requires.</rdfs:comment>
    </owl:ObjectProperty>
    


    <!-- http://purl.org/ontology/UniOn#hasAssessmentMethod -->

    <owl:ObjectProperty rdf:about="http://purl.org/ontology/UniOn#hasAssessmentMethod">
        <owl:inverseOf rdf:resource="http://purl.org/ontology/UniOn#isAssessmentMethodOf"/>
        <rdfs:domain rdf:resource="http://purl.org/ontology/UniOn#EducationalActivity"/>
        <rdfs:range rdf:resource="http://purl.org/ontology/UniOn#AssessmentMethod"/>
        <rdfs:comment>A property that relates an educational activity to a particular evaluation modality. Example of an assessment method include an oral or  writtem exam, the subsmission of a project or an eligibility.</rdfs:comment>
    </owl:ObjectProperty>
    


    <!-- http://purl.org/ontology/UniOn#hasCampus -->

    <owl:ObjectProperty rdf:about="http://purl.org/ontology/UniOn#hasCampus">
        <owl:inverseOf rdf:resource="http://purl.org/ontology/UniOn#isCampusOf"/>
        <rdfs:domain rdf:resource="http://purl.org/ontology/UniOn#DegreeProgramme"/>
        <rdfs:range rdf:resource="http://www.ontologydesignpatterns.org/ont/dul/DUL.owl#Place"/>
        <rdfs:comment>A property that associates the degree programme to the particular place where the university campus is located.</rdfs:comment>
    </owl:ObjectProperty>
    


    <!-- http://purl.org/ontology/UniOn#hasCurriculum -->

    <owl:ObjectProperty rdf:about="http://purl.org/ontology/UniOn#hasCurriculum">
        <owl:inverseOf rdf:resource="http://purl.org/ontology/UniOn#isCurriculumOf"/>
        <rdfs:domain rdf:resource="http://purl.org/ontology/UniOn#DegreeProgramme"/>
        <rdfs:range rdf:resource="http://purl.org/ontology/UniOn#Curriculum"/>
        <rdfs:comment>A property linking a degree programme to the curricula it offers.</rdfs:comment>
    </owl:ObjectProperty>
    


    <!-- http://purl.org/ontology/UniOn#hasEducationalActivity -->

    <owl:ObjectProperty rdf:about="http://purl.org/ontology/UniOn#hasEducationalActivity">
        <owl:inverseOf rdf:resource="http://purl.org/ontology/UniOn#isEducationalActivityOf"/>
        <rdfs:domain rdf:resource="http://purl.org/ontology/UniOn#DegreeProgramme"/>
        <rdfs:range rdf:resource="http://purl.org/ontology/UniOn#EducationalActivity"/>
        <rdfs:comment>A property that associates a degree programme to the educational activities it delivers.</rdfs:comment>
    </owl:ObjectProperty>
    


    <!-- http://purl.org/ontology/UniOn#hasPlaceOfTeaching -->

    <owl:ObjectProperty rdf:about="http://purl.org/ontology/UniOn#hasPlaceOfTeaching">
        <owl:inverseOf rdf:resource="http://purl.org/ontology/UniOn#isPlaceOfTeachingOf"/>
        <rdfs:domain rdf:resource="http://purl.org/ontology/UniOn#DegreeProgramme"/>
        <rdfs:range rdf:resource="http://www.ontologydesignpatterns.org/ont/dul/DUL.owl#Place"/>
        <rdfs:comment>A property that relates the degree programme to the place where its educational activities take place.</rdfs:comment>
    </owl:ObjectProperty>
    


    <!-- http://purl.org/ontology/UniOn#isAcademicFieldOf -->

    <owl:ObjectProperty rdf:about="http://purl.org/ontology/UniOn#isAcademicFieldOf">
        <rdfs:domain rdf:resource="http://purl.org/ontology/UniOn#AcademicField"/>
        <rdfs:range rdf:resource="http://purl.org/ontology/UniOn#DegreeProgramme"/>
        <rdfs:comment>A property describing the academic field to which a degree programme belongs.</rdfs:comment>
    </owl:ObjectProperty>
    


    <!-- http://purl.org/ontology/UniOn#isAccessTypeOf -->

    <owl:ObjectProperty rdf:about="http://purl.org/ontology/UniOn#isAccessTypeOf">
        <rdfs:domain rdf:resource="http://purl.org/ontology/UniOn#AccessType"/>
        <rdfs:range rdf:resource="http://purl.org/ontology/UniOn#DegreeProgramme"/>
        <rdfs:comment>A property indicating the modality of access a degree programme requires.</rdfs:comment>
    </owl:ObjectProperty>
    


    <!-- http://purl.org/ontology/UniOn#isAssessmentMethodOf -->

    <owl:ObjectProperty rdf:about="http://purl.org/ontology/UniOn#isAssessmentMethodOf">
        <rdfs:domain rdf:resource="http://purl.org/ontology/UniOn#AssessmentMethod"/>
        <rdfs:range rdf:resource="http://purl.org/ontology/UniOn#EducationalActivity"/>
        <rdfs:comment>A property expressing  the evaluation modality of an educational activity. Example of an assessment method include an oral or  writtem exam, the subsmission of a project or an eligibility.</rdfs:comment>
    </owl:ObjectProperty>
    


    <!-- http://purl.org/ontology/UniOn#isCampusOf -->

    <owl:ObjectProperty rdf:about="http://purl.org/ontology/UniOn#isCampusOf">
        <rdfs:domain rdf:resource="http://www.ontologydesignpatterns.org/ont/dul/DUL.owl#Place"/>
        <rdfs:range rdf:resource="http://purl.org/ontology/UniOn#DegreeProgramme"/>
        <rdfs:comment>A property indicating the place where the campus of a particular degree programme is located.</rdfs:comment>
    </owl:ObjectProperty>
    


    <!-- http://purl.org/ontology/UniOn#isCurriculumOf -->

    <owl:ObjectProperty rdf:about="http://purl.org/ontology/UniOn#isCurriculumOf">
        <rdfs:domain rdf:resource="http://purl.org/ontology/UniOn#Curriculum"/>
        <rdfs:range rdf:resource="http://purl.org/ontology/UniOn#DegreeProgramme"/>
        <rdfs:comment>A property that  indicates the curricula offered by the same degree programme.</rdfs:comment>
    </owl:ObjectProperty>
    


    <!-- http://purl.org/ontology/UniOn#isDeliveredBy -->

    <owl:ObjectProperty rdf:about="http://purl.org/ontology/UniOn#isDeliveredBy">
        <rdfs:domain rdf:resource="http://purl.org/ontology/UniOn#DegreeProgramme"/>
        <rdfs:range rdf:resource="http://purl.org/ontology/UniOn#ItalianPublicUniversity"/>
        <rdfs:comment>A property indicating the degree programmes delivered by an italian public university.</rdfs:comment>
    </owl:ObjectProperty>
    


    <!-- http://purl.org/ontology/UniOn#isEducationalActivityOf -->

    <owl:ObjectProperty rdf:about="http://purl.org/ontology/UniOn#isEducationalActivityOf">
        <rdfs:domain rdf:resource="http://purl.org/ontology/UniOn#EducationalActivity"/>
        <rdfs:range rdf:resource="http://purl.org/ontology/UniOn#DegreeProgramme"/>
        <rdfs:comment>A property indicating the educational activity delivered by a degree programme.</rdfs:comment>
    </owl:ObjectProperty>
    


    <!-- http://purl.org/ontology/UniOn#isManagedBy -->

    <owl:ObjectProperty rdf:about="http://purl.org/ontology/UniOn#isManagedBy">
        <owl:inverseOf rdf:resource="http://purl.org/ontology/UniOn#manages"/>
        <rdfs:domain rdf:resource="http://purl.org/ontology/UniOn#DegreeProgramme"/>
        <rdfs:range rdf:resource="http://purl.org/ontology/UniOn#Department"/>
        <rdfs:comment>A property indicating the university department managed by a public italian university.</rdfs:comment>
    </owl:ObjectProperty>
    


    <!-- http://purl.org/ontology/UniOn#isOfferedBy -->

    <owl:ObjectProperty rdf:about="http://purl.org/ontology/UniOn#isOfferedBy">
        <owl:inverseOf rdf:resource="http://purl.org/ontology/UniOn#offers"/>
        <rdfs:domain rdf:resource="http://purl.org/ontology/UniOn#EducationalActivity"/>
        <rdfs:range rdf:resource="http://purl.org/ontology/UniOn#ItalianPublicUniversity"/>
        <rdfs:comment>Superproperty that joins an educational activity to a particular italian public university via the degree programme.</rdfs:comment>
    </owl:ObjectProperty>
    


    <!-- http://purl.org/ontology/UniOn#isPlaceOfTeachingOf -->

    <owl:ObjectProperty rdf:about="http://purl.org/ontology/UniOn#isPlaceOfTeachingOf">
        <rdfs:domain rdf:resource="http://www.ontologydesignpatterns.org/ont/dul/DUL.owl#Place"/>
        <rdfs:range rdf:resource="http://purl.org/ontology/UniOn#DegreeProgramme"/>
        <rdfs:comment>A property that indicates the location where the degree programme&apos;s educational acitvities take place.</rdfs:comment>
    </owl:ObjectProperty>
    


    <!-- http://purl.org/ontology/UniOn#isReleasedBy -->

    <owl:ObjectProperty rdf:about="http://purl.org/ontology/UniOn#isReleasedBy">
        <owl:inverseOf rdf:resource="http://purl.org/ontology/UniOn#releases"/>
        <rdfs:domain rdf:resource="http://purl.org/ontology/UniOn#Qualification"/>
        <rdfs:range rdf:resource="http://purl.org/ontology/UniOn#DegreeProgramme"/>
        <rdfs:comment>A property expressing the official qualification released to the student after the completion of a degree programme.</rdfs:comment>
    </owl:ObjectProperty>
    


    <!-- http://purl.org/ontology/UniOn#manages -->

    <owl:ObjectProperty rdf:about="http://purl.org/ontology/UniOn#manages">
        <rdfs:domain rdf:resource="http://purl.org/ontology/UniOn#Department"/>
        <rdfs:range rdf:resource="http://purl.org/ontology/UniOn#DegreeProgramme"/>
        <rdfs:comment>A property that associates the university deparment to the degree programme it manages.</rdfs:comment>
    </owl:ObjectProperty>
    


    <!-- http://purl.org/ontology/UniOn#offers -->

    <owl:ObjectProperty rdf:about="http://purl.org/ontology/UniOn#offers">
        <rdfs:domain rdf:resource="http://purl.org/ontology/UniOn#ItalianPublicUniversity"/>
        <rdfs:range rdf:resource="http://purl.org/ontology/UniOn#EducationalActivity"/>
        <owl:propertyChainAxiom rdf:parseType="Collection">
            <rdf:Description rdf:about="http://purl.org/ontology/UniOn#delivers"/>
            <rdf:Description rdf:about="http://purl.org/ontology/UniOn#hasEducationalActivity"/>
        </owl:propertyChainAxiom>
        <rdfs:comment>Superproperty that joins an italian public university with a particular educational activity via the degree programme.</rdfs:comment>
    </owl:ObjectProperty>
    


    <!-- http://purl.org/ontology/UniOn#releases -->

    <owl:ObjectProperty rdf:about="http://purl.org/ontology/UniOn#releases">
        <rdfs:domain rdf:resource="http://purl.org/ontology/UniOn#DegreeProgramme"/>
        <rdfs:range rdf:resource="http://purl.org/ontology/UniOn#Qualification"/>
        <rdfs:comment>A property that relates the degree programme to the official qualification the students receives after completing the study programme.</rdfs:comment>
    </owl:ObjectProperty>
    


    <!-- http://www.ontologydesignpatterns.org/ont/dul/DUL.owl#hasPart -->

    <owl:ObjectProperty rdf:about="http://www.ontologydesignpatterns.org/ont/dul/DUL.owl#hasPart">
        <owl:inverseOf rdf:resource="http://www.ontologydesignpatterns.org/ont/dul/DUL.owl#isPartOf"/>
        <rdfs:domain rdf:resource="http://purl.org/ontology/UniOn#ItalianPublicUniversity"/>
        <rdfs:range rdf:resource="http://purl.org/ontology/UniOn#Department"/>
        <rdfs:comment>A property indicating that one entity (the university) includes another entity (the department).</rdfs:comment>
    </owl:ObjectProperty>
    


    <!-- http://www.ontologydesignpatterns.org/ont/dul/DUL.owl#isPartOf -->

    <owl:ObjectProperty rdf:about="http://www.ontologydesignpatterns.org/ont/dul/DUL.owl#isPartOf">
        <rdfs:domain rdf:resource="http://purl.org/ontology/UniOn#Department"/>
        <rdfs:range rdf:resource="http://purl.org/ontology/UniOn#ItalianPublicUniversity"/>
        <rdfs:comment>A property indicating that one entity (the department) is a part of another entity (the university).</rdfs:comment>
    </owl:ObjectProperty>
    


    <!-- 
    ///////////////////////////////////////////////////////////////////////////////////////
    //
    // Data properties
    //
    ///////////////////////////////////////////////////////////////////////////////////////
     -->

    


    <!-- http://purl.org/ontology/UniOn#hasAcademicYear -->

    <owl:DatatypeProperty rdf:about="http://purl.org/ontology/UniOn#hasAcademicYear">
        <rdfs:domain rdf:resource="http://purl.org/ontology/UniOn#DegreeProgramme"/>
        <rdfs:comment>The period in which the degree programme carries its traning activity.</rdfs:comment>
    </owl:DatatypeProperty>
    


    <!-- http://purl.org/ontology/UniOn#hasCfu -->

    <owl:DatatypeProperty rdf:about="http://purl.org/ontology/UniOn#hasCfu">
        <rdfs:domain rdf:resource="http://purl.org/ontology/UniOn#EducationalActivity"/>
        <rdfs:comment>The CFUs of a particular educational activity. CFUs (university formative credits) are a numerical measure of the workload for each exam or activity.</rdfs:comment>
    </owl:DatatypeProperty>
    


    <!-- http://purl.org/ontology/UniOn#hasDegreeClass -->

    <owl:DatatypeProperty rdf:about="http://purl.org/ontology/UniOn#hasDegreeClass">
        <rdfs:subPropertyOf rdf:resource="http://purl.org/ontology/UniOn#hasIdentifier"/>
        <rdfs:domain rdf:resource="http://purl.org/ontology/UniOn#DegreeProgramme"/>
        <rdfs:comment>The degree class (a unique code) of each degree programme. (E.g. LM-43 - Information technology methods for the humanities)</rdfs:comment>
    </owl:DatatypeProperty>
    


    <!-- http://purl.org/ontology/UniOn#hasIdentifier -->

    <owl:DatatypeProperty rdf:about="http://purl.org/ontology/UniOn#hasIdentifier">
        <rdfs:domain>
            <owl:Class>
                <owl:unionOf rdf:parseType="Collection">
                    <rdf:Description rdf:about="http://purl.org/ontology/UniOn#DegreeProgramme"/>
                    <rdf:Description rdf:about="http://purl.org/ontology/UniOn#EducationalActivity"/>
                </owl:unionOf>
            </owl:Class>
        </rdfs:domain>
        <rdfs:comment>A property that expresses the particular identifiers used by the italian university system to describe and identify degree programmes and educational activities. (E.g. Degree Class, Ssd and Teaching Code)</rdfs:comment>
    </owl:DatatypeProperty>
    


    <!-- http://purl.org/ontology/UniOn#hasSsd -->

    <owl:DatatypeProperty rdf:about="http://purl.org/ontology/UniOn#hasSsd">
        <rdfs:subPropertyOf rdf:resource="http://purl.org/ontology/UniOn#hasIdentifier"/>
        <rdfs:domain rdf:resource="http://purl.org/ontology/UniOn#EducationalActivity"/>
        <rdfs:comment>The SSD of an educational activity. SSD stands for ‘scientific-disciplinary sectors’: they point to the disciplinary areas to which each educational activity belongs to.</rdfs:comment>
    </owl:DatatypeProperty>
    


    <!-- http://purl.org/ontology/UniOn#hasTeachingCode -->

    <owl:DatatypeProperty rdf:about="http://purl.org/ontology/UniOn#hasTeachingCode">
        <rdfs:subPropertyOf rdf:resource="http://purl.org/ontology/UniOn#hasIdentifier"/>
        <rdfs:domain rdf:resource="http://purl.org/ontology/UniOn#EducationalActivity"/>
        <rdfs:comment>A numerical code chosen by each university to univocally identify its educational activities.</rdfs:comment>
    </owl:DatatypeProperty>
    


    <!-- http://purl.org/ontology/UniOn#hasTeachingLanguage -->

    <owl:DatatypeProperty rdf:about="http://purl.org/ontology/UniOn#hasTeachingLanguage">
        <rdfs:domain rdf:resource="http://purl.org/ontology/UniOn#DegreeProgramme"/>
        <rdfs:comment>The language in which the degree programme is taught.</rdfs:comment>
    </owl:DatatypeProperty>
    


    <!-- http://purl.org/ontology/UniOn#hasUrl -->

    <owl:DatatypeProperty rdf:about="http://purl.org/ontology/UniOn#hasUrl">
        <rdfs:domain rdf:resource="http://purl.org/ontology/UniOn#DegreeProgramme"/>
        <rdfs:comment>The Url pointing to the website of the degree programme.</rdfs:comment>
    </owl:DatatypeProperty>
    


    <!-- http://purl.org/ontology/UniOn#hasYearsOfDuration -->

    <owl:DatatypeProperty rdf:about="http://purl.org/ontology/UniOn#hasYearsOfDuration">
        <rdfs:domain rdf:resource="http://purl.org/ontology/UniOn#DegreeProgramme"/>
        <rdfs:comment>The duration of a degree programme.</rdfs:comment>
    </owl:DatatypeProperty>
    


    <!-- http://purl.org/ontology/UniOn#isCompulsory -->

    <owl:DatatypeProperty rdf:about="http://purl.org/ontology/UniOn#isCompulsory">
        <rdfs:domain rdf:resource="http://purl.org/ontology/UniOn#EducationalActivity"/>
        <rdfs:comment>The property indicates if an educational activity is compulsory or not.</rdfs:comment>
    </owl:DatatypeProperty>
    


    <!-- 
    ///////////////////////////////////////////////////////////////////////////////////////
    //
    // Classes
    //
    ///////////////////////////////////////////////////////////////////////////////////////
     -->

    


    <!-- http://purl.org/ontology/UniOn#AcademicField -->

    <owl:Class rdf:about="http://purl.org/ontology/UniOn#AcademicField">
        <rdfs:comment>The fields involved in an educational offer of a university (e.g. Humanities, Business, Sciences etc.).</rdfs:comment>
    </owl:Class>
    


    <!-- http://purl.org/ontology/UniOn#AccessType -->

    <owl:Class rdf:about="http://purl.org/ontology/UniOn#AccessType">
        <owl:equivalentClass>
            <owl:Class>
                <owl:oneOf rdf:parseType="Collection">
                    <rdf:Description rdf:about="http://purl.org/ontology/UniOn#LimitedAccess"/>
                    <rdf:Description rdf:about="http://purl.org/ontology/UniOn#OpenAccess"/>
                </owl:oneOf>
            </owl:Class>
        </owl:equivalentClass>
        <owl:equivalentClass>
            <owl:Restriction>
                <owl:onProperty rdf:resource="http://purl.org/ontology/UniOn#isAccessTypeOf"/>
                <owl:someValuesFrom rdf:resource="http://purl.org/ontology/UniOn#DegreeProgramme"/>
            </owl:Restriction>
        </owl:equivalentClass>
        <rdfs:comment>The modality of  access the degree courses require.</rdfs:comment>
    </owl:Class>
    


    <!-- http://purl.org/ontology/UniOn#AssessmentMethod -->

    <owl:Class rdf:about="http://purl.org/ontology/UniOn#AssessmentMethod">
        <owl:equivalentClass>
            <owl:Class>
                <owl:oneOf rdf:parseType="Collection">
                    <rdf:Description rdf:about="http://purl.org/ontology/UniOn#Eligibility"/>
                    <rdf:Description rdf:about="http://purl.org/ontology/UniOn#OralExam"/>
                    <rdf:Description rdf:about="http://purl.org/ontology/UniOn#Project"/>
                    <rdf:Description rdf:about="http://purl.org/ontology/UniOn#WrittenExam"/>
                </owl:oneOf>
            </owl:Class>
        </owl:equivalentClass>
        <owl:equivalentClass>
            <owl:Restriction>
                <owl:onProperty rdf:resource="http://purl.org/ontology/UniOn#isAssessmentMethodOf"/>
                <owl:someValuesFrom rdf:resource="http://purl.org/ontology/UniOn#EducationalActivity"/>
            </owl:Restriction>
        </owl:equivalentClass>
        <rdfs:comment>The evaluation modality for each educational activity (e.g. Written exam, Oral exam etc.)</rdfs:comment>
    </owl:Class>
    


    <!-- http://purl.org/ontology/UniOn#BachelorDegree -->

    <owl:Class rdf:about="http://purl.org/ontology/UniOn#BachelorDegree">
        <rdfs:subClassOf rdf:resource="http://purl.org/ontology/UniOn#DegreeProgramme"/>
        <rdfs:comment>The bachelor degree (180 CFU) is a first cycle degree whose normative time to completion is three years.</rdfs:comment>
    </owl:Class>
    


    <!-- http://purl.org/ontology/UniOn#Course -->

    <owl:Class rdf:about="http://purl.org/ontology/UniOn#Course">
        <rdfs:subClassOf rdf:resource="http://purl.org/ontology/UniOn#EducationalActivity"/>
        <rdfs:comment>A university course is made up of a set of lessons held by one teacher or several teachers.</rdfs:comment>
    </owl:Class>
    


    <!-- http://purl.org/ontology/UniOn#Curriculum -->

    <owl:Class rdf:about="http://purl.org/ontology/UniOn#Curriculum">
        <rdfs:comment>The same degree program can have multiple curricula that include different  training activities. E.g.  For the degree course in &quot;Literature&quot;, it is possible to choose between the curriculum in Classical or Modern studies.</rdfs:comment>
    </owl:Class>
    


    <!-- http://purl.org/ontology/UniOn#DegreeProgramme -->

    <owl:Class rdf:about="http://purl.org/ontology/UniOn#DegreeProgramme">
        <owl:equivalentClass>
            <owl:Class>
                <owl:intersectionOf rdf:parseType="Collection">
                    <owl:Restriction>
                        <owl:onProperty rdf:resource="http://purl.org/ontology/UniOn#hasAcademicField"/>
                        <owl:someValuesFrom rdf:resource="http://purl.org/ontology/UniOn#AcademicField"/>
                    </owl:Restriction>
                    <owl:Restriction>
                        <owl:onProperty rdf:resource="http://purl.org/ontology/UniOn#hasCampus"/>
                        <owl:someValuesFrom rdf:resource="http://www.ontologydesignpatterns.org/ont/dul/DUL.owl#Place"/>
                    </owl:Restriction>
                    <owl:Restriction>
                        <owl:onProperty rdf:resource="http://purl.org/ontology/UniOn#hasPlaceOfTeaching"/>
                        <owl:someValuesFrom rdf:resource="http://www.ontologydesignpatterns.org/ont/dul/DUL.owl#Place"/>
                    </owl:Restriction>
                    <owl:Restriction>
                        <owl:onProperty rdf:resource="http://purl.org/ontology/UniOn#isDeliveredBy"/>
                        <owl:someValuesFrom rdf:resource="http://purl.org/ontology/UniOn#ItalianPublicUniversity"/>
                    </owl:Restriction>
                    <owl:Restriction>
                        <owl:onProperty rdf:resource="http://purl.org/ontology/UniOn#isManagedBy"/>
                        <owl:someValuesFrom rdf:resource="http://purl.org/ontology/UniOn#Department"/>
                    </owl:Restriction>
                    <owl:Restriction>
                        <owl:onProperty rdf:resource="http://purl.org/ontology/UniOn#releases"/>
                        <owl:someValuesFrom rdf:resource="http://purl.org/ontology/UniOn#Qualification"/>
                    </owl:Restriction>
                    <owl:Restriction>
                        <owl:onProperty rdf:resource="http://purl.org/ontology/UniOn#hasCurriculum"/>
                        <owl:minQualifiedCardinality rdf:datatype="http://www.w3.org/2001/XMLSchema#nonNegativeInteger">0</owl:minQualifiedCardinality>
                        <owl:onClass rdf:resource="http://purl.org/ontology/UniOn#Curriculum"/>
                    </owl:Restriction>
                    <owl:Restriction>
                        <owl:onProperty rdf:resource="http://purl.org/ontology/UniOn#hasEducationalActivity"/>
                        <owl:minQualifiedCardinality rdf:datatype="http://www.w3.org/2001/XMLSchema#nonNegativeInteger">1</owl:minQualifiedCardinality>
                        <owl:onClass rdf:resource="http://purl.org/ontology/UniOn#EducationalActivity"/>
                    </owl:Restriction>
                    <owl:Restriction>
                        <owl:onProperty rdf:resource="http://purl.org/ontology/UniOn#hasAccessType"/>
                        <owl:qualifiedCardinality rdf:datatype="http://www.w3.org/2001/XMLSchema#nonNegativeInteger">1</owl:qualifiedCardinality>
                        <owl:onClass rdf:resource="http://purl.org/ontology/UniOn#AccessType"/>
                    </owl:Restriction>
                </owl:intersectionOf>
            </owl:Class>
        </owl:equivalentClass>
        <rdfs:comment>A university-specific degree programme referring to a more general academic field (e.g. Digital Humanities and Digital Knowledge degree programme at UniBo)</rdfs:comment>
    </owl:Class>
    


    <!-- http://purl.org/ontology/UniOn#Department -->

    <owl:Class rdf:about="http://purl.org/ontology/UniOn#Department">
        <owl:equivalentClass>
            <owl:Class>
                <owl:intersectionOf rdf:parseType="Collection">
                    <owl:Restriction>
                        <owl:onProperty rdf:resource="http://purl.org/ontology/UniOn#manages"/>
                        <owl:someValuesFrom rdf:resource="http://purl.org/ontology/UniOn#DegreeProgramme"/>
                    </owl:Restriction>
                    <owl:Restriction>
                        <owl:onProperty rdf:resource="http://www.ontologydesignpatterns.org/ont/dul/DUL.owl#isPartOf"/>
                        <owl:someValuesFrom rdf:resource="http://purl.org/ontology/UniOn#ItalianPublicUniversity"/>
                    </owl:Restriction>
                </owl:intersectionOf>
            </owl:Class>
        </owl:equivalentClass>
        <rdfs:comment>Organizational structure that within Italian universities promotes and coordinates the activities of one or more sectors of scientific research that are homogeneous in terms of aims and methods.</rdfs:comment>
    </owl:Class>
    


    <!-- http://purl.org/ontology/UniOn#EducationalActivity -->

    <owl:Class rdf:about="http://purl.org/ontology/UniOn#EducationalActivity">
        <rdfs:comment>Any kind of educational activity: exams, internships, laboratories, seminars etc.</rdfs:comment>
    </owl:Class>
    


    <!-- http://purl.org/ontology/UniOn#FinalTest -->

    <owl:Class rdf:about="http://purl.org/ontology/UniOn#FinalTest">
        <rdfs:subClassOf rdf:resource="http://purl.org/ontology/UniOn#EducationalActivity"/>
        <rdfs:comment>The final examination: it consists in producing a dissertation on a topic that is consistent with the learning objectives of the degree programme, drafted in an original manner under the guidance of a supervising professor</rdfs:comment>
    </owl:Class>
    


    <!-- http://purl.org/ontology/UniOn#InternationalDegree -->

    <owl:Class rdf:about="http://purl.org/ontology/UniOn#InternationalDegree">
        <rdfs:subClassOf rdf:resource="http://purl.org/ontology/UniOn#DegreeProgramme"/>
        <rdfs:comment>A degree programme delivered in a foreign language.</rdfs:comment>
    </owl:Class>
    


    <!-- http://purl.org/ontology/UniOn#Internship -->

    <owl:Class rdf:about="http://purl.org/ontology/UniOn#Internship">
        <rdfs:subClassOf rdf:resource="http://purl.org/ontology/UniOn#EducationalActivity"/>
        <rdfs:comment>An internship is a period of work experience offered by an organization or an institution for a limited period of time.</rdfs:comment>
    </owl:Class>
    


    <!-- http://purl.org/ontology/UniOn#ItalianPublicUniversity -->

    <owl:Class rdf:about="http://purl.org/ontology/UniOn#ItalianPublicUniversity">
        <owl:equivalentClass>
            <owl:Class>
                <owl:intersectionOf rdf:parseType="Collection">
                    <owl:Restriction>
                        <owl:onProperty rdf:resource="http://purl.org/ontology/UniOn#delivers"/>
                        <owl:minQualifiedCardinality rdf:datatype="http://www.w3.org/2001/XMLSchema#nonNegativeInteger">1</owl:minQualifiedCardinality>
                        <owl:onClass rdf:resource="http://purl.org/ontology/UniOn#DegreeProgramme"/>
                    </owl:Restriction>
                    <owl:Restriction>
                        <owl:onProperty rdf:resource="http://www.ontologydesignpatterns.org/ont/dul/DUL.owl#hasPart"/>
                        <owl:minQualifiedCardinality rdf:datatype="http://www.w3.org/2001/XMLSchema#nonNegativeInteger">1</owl:minQualifiedCardinality>
                        <owl:onClass rdf:resource="http://purl.org/ontology/UniOn#Department"/>
                    </owl:Restriction>
                </owl:intersectionOf>
            </owl:Class>
        </owl:equivalentClass>
        <rdfs:comment>A specific public italian university (e.g. Unibo)</rdfs:comment>
    </owl:Class>
    


    <!-- http://purl.org/ontology/UniOn#Laboratory -->

    <owl:Class rdf:about="http://purl.org/ontology/UniOn#Laboratory">
        <rdfs:subClassOf rdf:resource="http://purl.org/ontology/UniOn#EducationalActivity"/>
        <rdfs:comment>A laboratory deals with specific topics related to the degree programme and involves practical activities.</rdfs:comment>
    </owl:Class>
    


    <!-- http://purl.org/ontology/UniOn#LimitedAccessDegree -->

    <owl:Class rdf:about="http://purl.org/ontology/UniOn#LimitedAccessDegree">
        <owl:equivalentClass>
            <owl:Class>
                <owl:intersectionOf rdf:parseType="Collection">
                    <rdf:Description rdf:about="http://purl.org/ontology/UniOn#DegreeProgramme"/>
                    <owl:Restriction>
                        <owl:onProperty rdf:resource="http://purl.org/ontology/UniOn#hasAccessType"/>
                        <owl:hasValue rdf:resource="http://purl.org/ontology/UniOn#LimitedAccess"/>
                    </owl:Restriction>
                </owl:intersectionOf>
            </owl:Class>
        </owl:equivalentClass>
        <owl:disjointWith rdf:resource="http://purl.org/ontology/UniOn#OpenAccessDegree"/>
        <rdfs:comment>A degree programme in which places available are limited and enrollment is only possible after overcoming a selection.</rdfs:comment>
    </owl:Class>
    


    <!-- http://purl.org/ontology/UniOn#MasterDegree -->

    <owl:Class rdf:about="http://purl.org/ontology/UniOn#MasterDegree">
        <rdfs:subClassOf rdf:resource="http://purl.org/ontology/UniOn#DegreeProgramme"/>
        <rdfs:comment>The master degree is a second cycle degree (120 CFU) which can be earned in a two-year programme after the bachelor degree.</rdfs:comment>
    </owl:Class>
    


    <!-- http://purl.org/ontology/UniOn#OpenAccessDegree -->

    <owl:Class rdf:about="http://purl.org/ontology/UniOn#OpenAccessDegree">
        <owl:equivalentClass>
            <owl:Class>
                <owl:intersectionOf rdf:parseType="Collection">
                    <rdf:Description rdf:about="http://purl.org/ontology/UniOn#DegreeProgramme"/>
                    <owl:Restriction>
                        <owl:onProperty rdf:resource="http://purl.org/ontology/UniOn#hasAccessType"/>
                        <owl:hasValue rdf:resource="http://purl.org/ontology/UniOn#OpenAccess"/>
                    </owl:Restriction>
                </owl:intersectionOf>
            </owl:Class>
        </owl:equivalentClass>
        <rdfs:comment>A degree programme in which there is no maximum number of available places and enrollment does not entail passing through a selection. An entry test, however may be required.</rdfs:comment>
    </owl:Class>
    


    <!-- http://purl.org/ontology/UniOn#Qualification -->

    <owl:Class rdf:about="http://purl.org/ontology/UniOn#Qualification">
        <owl:equivalentClass>
            <owl:Class>
                <owl:oneOf rdf:parseType="Collection">
                    <rdf:Description rdf:about="http://purl.org/ontology/UniOn#JointQualification"/>
                    <rdf:Description rdf:about="http://purl.org/ontology/UniOn#MultipleQualification"/>
                    <rdf:Description rdf:about="http://purl.org/ontology/UniOn#SingleQualification"/>
                </owl:oneOf>
            </owl:Class>
        </owl:equivalentClass>
        <owl:equivalentClass>
            <owl:Restriction>
                <owl:onProperty rdf:resource="http://purl.org/ontology/UniOn#isReleasedBy"/>
                <owl:someValuesFrom rdf:resource="http://purl.org/ontology/UniOn#ItalianPublicUniversity"/>
            </owl:Restriction>
        </owl:equivalentClass>
        <rdfs:comment>A qualification (or degree) is the official record of achievement you receive after completing a programme of study. There are several types of qualifications varying in level of study and length of time.</rdfs:comment>
    </owl:Class>
    


    <!-- http://purl.org/ontology/UniOn#Seminar -->

    <owl:Class rdf:about="http://purl.org/ontology/UniOn#Seminar">
        <rdfs:subClassOf rdf:resource="http://purl.org/ontology/UniOn#EducationalActivity"/>
        <rdfs:comment>University seminars deal with a specific topic within a discipline from several points of view, involving specialists both internal and external to the university encouraging students to actively participate.</rdfs:comment>
    </owl:Class>
    


    <!-- http://purl.org/ontology/UniOn#SingleCycleDegree -->

    <owl:Class rdf:about="http://purl.org/ontology/UniOn#SingleCycleDegree">
        <rdfs:subClassOf rdf:resource="http://purl.org/ontology/UniOn#DegreeProgramme"/>
        <rdfs:comment>The single cycle degree is a five or six year degree (300 or 360 CFU), which does not require a previous first cycle degree for the admission</rdfs:comment>
    </owl:Class>
    


    <!-- http://www.ontologydesignpatterns.org/ont/dul/DUL.owl#Place -->

    <owl:Class rdf:about="http://www.ontologydesignpatterns.org/ont/dul/DUL.owl#Place">
        <rdfs:comment>Place where the educational activity takes place and where the university campus is located.</rdfs:comment>
    </owl:Class>
    


    <!-- 
    ///////////////////////////////////////////////////////////////////////////////////////
    //
    // Individuals
    //
    ///////////////////////////////////////////////////////////////////////////////////////
     -->

    


    <!-- http://purl.org/ontology/UniOn#Eligibility -->

    <owl:NamedIndividual rdf:about="http://purl.org/ontology/UniOn#Eligibility">
        <rdf:type rdf:resource="http://purl.org/ontology/UniOn#AssessmentMethod"/>
        <rdfs:comment>Exam without grade (with eligible or not eligible result) which assesses the candidate competencies.</rdfs:comment>
        <rdfs:label>Eligibility</rdfs:label>
    </owl:NamedIndividual>
    


    <!-- http://purl.org/ontology/UniOn#JointQualification -->

    <owl:NamedIndividual rdf:about="http://purl.org/ontology/UniOn#JointQualification">
        <rdf:type rdf:resource="http://purl.org/ontology/UniOn#Qualification"/>
        <rdfs:comment>Joint qualification means obtaining a single qualification recognised and validated by all the institutions running the joint programme.</rdfs:comment>
        <rdfs:label>Joint Qualification</rdfs:label>
    </owl:NamedIndividual>
    


    <!-- http://purl.org/ontology/UniOn#LimitedAccess -->

    <owl:NamedIndividual rdf:about="http://purl.org/ontology/UniOn#LimitedAccess">
        <rdf:type rdf:resource="http://purl.org/ontology/UniOn#AccessType"/>
        <rdfs:comment>The type of access indicating that the places available are limited and enrollment is only possible after overcoming a selection.</rdfs:comment>
        <rdfs:label>Limited Access</rdfs:label>
    </owl:NamedIndividual>
    


    <!-- http://purl.org/ontology/UniOn#MultipleQualification -->

    <owl:NamedIndividual rdf:about="http://purl.org/ontology/UniOn#MultipleQualification">
        <rdf:type rdf:resource="http://purl.org/ontology/UniOn#Qualification"/>
        <rdfs:comment>Double or multiple qualifications implies that, at the end of the programme, students obtain not only a degree from their home university but also the academic qualifications from the other participating universities where they have obtained learning credits</rdfs:comment>
        <rdfs:label>Multiple Qualification</rdfs:label>
    </owl:NamedIndividual>
    


    <!-- http://purl.org/ontology/UniOn#OpenAccess -->

    <owl:NamedIndividual rdf:about="http://purl.org/ontology/UniOn#OpenAccess">
        <rdf:type rdf:resource="http://purl.org/ontology/UniOn#AccessType"/>
        <rdfs:comment>The type of access indicating that there is no maximum number of available places and enrollment does not entail passing through a selection. An entry test, however may be required.</rdfs:comment>
        <rdfs:label>Open Access</rdfs:label>
    </owl:NamedIndividual>
    


    <!-- http://purl.org/ontology/UniOn#OralExam -->

    <owl:NamedIndividual rdf:about="http://purl.org/ontology/UniOn#OralExam">
        <rdf:type rdf:resource="http://purl.org/ontology/UniOn#AssessmentMethod"/>
        <rdfs:comment>An examination in spoken form to show how well a student has understood the material studied in the program.</rdfs:comment>
        <rdfs:label>Oral Exam</rdfs:label>
    </owl:NamedIndividual>
    


    <!-- http://purl.org/ontology/UniOn#Project -->

    <owl:NamedIndividual rdf:about="http://purl.org/ontology/UniOn#Project">
        <rdf:type rdf:resource="http://purl.org/ontology/UniOn#AssessmentMethod"/>
        <rdfs:comment>Project-based assessments are an alternative to tests that allow students to engage with their learning in more concrete ways. Instead of merely studying theory, a hands-on project asks students to apply what they&apos;ve learned to an in-depth exploration of a topic.</rdfs:comment>
        <rdfs:label>Project</rdfs:label>
    </owl:NamedIndividual>
    


    <!-- http://purl.org/ontology/UniOn#SingleQualification -->

    <owl:NamedIndividual rdf:about="http://purl.org/ontology/UniOn#SingleQualification">
        <rdf:type rdf:resource="http://purl.org/ontology/UniOn#Qualification"/>
        <rdfs:comment>A single qualification issued by the university.</rdfs:comment>
        <rdfs:label>Single Qualification</rdfs:label>
    </owl:NamedIndividual>
    


    <!-- http://purl.org/ontology/UniOn#WrittenExam -->

    <owl:NamedIndividual rdf:about="http://purl.org/ontology/UniOn#WrittenExam">
        <rdf:type rdf:resource="http://purl.org/ontology/UniOn#AssessmentMethod"/>
        <rdfs:comment>An assessment method that requires the student to answer some questions in writing (or electronically).</rdfs:comment>
        <rdfs:label>Written Exam</rdfs:label>
    </owl:NamedIndividual>
    


    <!-- 
    ///////////////////////////////////////////////////////////////////////////////////////
    //
    // General axioms
    //
    ///////////////////////////////////////////////////////////////////////////////////////
     -->

    <rdf:Description>
        <rdf:type rdf:resource="http://www.w3.org/2002/07/owl#AllDisjointClasses"/>
        <owl:members rdf:parseType="Collection">
            <rdf:Description rdf:about="http://purl.org/ontology/UniOn#AcademicField"/>
            <rdf:Description rdf:about="http://purl.org/ontology/UniOn#AccessType"/>
            <rdf:Description rdf:about="http://purl.org/ontology/UniOn#AssessmentMethod"/>
            <rdf:Description rdf:about="http://purl.org/ontology/UniOn#Curriculum"/>
            <rdf:Description rdf:about="http://purl.org/ontology/UniOn#DegreeProgramme"/>
            <rdf:Description rdf:about="http://purl.org/ontology/UniOn#Department"/>
            <rdf:Description rdf:about="http://purl.org/ontology/UniOn#EducationalActivity"/>
            <rdf:Description rdf:about="http://purl.org/ontology/UniOn#ItalianPublicUniversity"/>
            <rdf:Description rdf:about="http://purl.org/ontology/UniOn#Qualification"/>
            <rdf:Description rdf:about="http://www.ontologydesignpatterns.org/ont/dul/DUL.owl#Place"/>
        </owl:members>
    </rdf:Description>
    <rdf:Description>
        <rdf:type rdf:resource="http://www.w3.org/2002/07/owl#AllDisjointClasses"/>
        <owl:members rdf:parseType="Collection">
            <rdf:Description rdf:about="http://purl.org/ontology/UniOn#BachelorDegree"/>
            <rdf:Description rdf:about="http://purl.org/ontology/UniOn#MasterDegree"/>
            <rdf:Description rdf:about="http://purl.org/ontology/UniOn#SingleCycleDegree"/>
        </owl:members>
    </rdf:Description>
    <rdf:Description>
        <rdf:type rdf:resource="http://www.w3.org/2002/07/owl#AllDisjointClasses"/>
        <owl:members rdf:parseType="Collection">
            <rdf:Description rdf:about="http://purl.org/ontology/UniOn#Course"/>
            <rdf:Description rdf:about="http://purl.org/ontology/UniOn#Internship"/>
            <rdf:Description rdf:about="http://purl.org/ontology/UniOn#Laboratory"/>
            <rdf:Description rdf:about="http://purl.org/ontology/UniOn#Seminar"/>
        </owl:members>
    </rdf:Description>
    <rdf:Description>
        <rdf:type rdf:resource="http://www.w3.org/2002/07/owl#AllDifferent"/>
        <owl:distinctMembers rdf:parseType="Collection">
            <rdf:Description rdf:about="http://purl.org/ontology/UniOn#Eligibility"/>
            <rdf:Description rdf:about="http://purl.org/ontology/UniOn#JointQualification"/>
            <rdf:Description rdf:about="http://purl.org/ontology/UniOn#LimitedAccess"/>
            <rdf:Description rdf:about="http://purl.org/ontology/UniOn#MultipleQualification"/>
            <rdf:Description rdf:about="http://purl.org/ontology/UniOn#OpenAccess"/>
            <rdf:Description rdf:about="http://purl.org/ontology/UniOn#OralExam"/>
            <rdf:Description rdf:about="http://purl.org/ontology/UniOn#Project"/>
            <rdf:Description rdf:about="http://purl.org/ontology/UniOn#SingleQualification"/>
            <rdf:Description rdf:about="http://purl.org/ontology/UniOn#WrittenExam"/>
        </owl:distinctMembers>
    </rdf:Description>
</rdf:RDF>



<!-- Generated by the OWL API (version 4.5.9.2019-02-01T07:24:44Z) https://github.com/owlcs/owlapi -->

